src/Narcissus/BinLib.v
@@ -14,6 +14,60 @@ Require Export
 
 Global Instance ByteStringQueueMonoid : Monoid ByteString := ByteStringQueueMonoid.
 
+Lemma CorrectAlignedDecoder2CorrectDecoder
+      {A} {cache : Cache.Cache}
+      Invariant
+      (FormatSpec : Specs.FormatM A _)
+      (decoder : CorrectAlignedDecoderFor Invariant FormatSpec)
+  : Specs.CorrectDecoderFor Invariant FormatSpec.
+Proof.
+  eexists (projT1 (projT2 decoder)).
+  abstract (destruct decoder as [aligned_decoder [ [decoder Inv] ? ] ]; simpl in *;
+            intuition eauto).
+Defined.
+
+Lemma CorrectAlignedEncoder2CorrectEncoder
+      {A} {cache : Cache.Cache}
+      (FormatSpec : Specs.FormatM A _)
+      (encoder : CorrectAlignedEncoderFor FormatSpec)
+  : Specs.CorrectEncoderFor FormatSpec.
+Proof.
+  eexists (projT1 (projT2 encoder)); split; intros;
+    destruct encoder as [aligned_encoder [encoder [encoder_OK [padding_OK encoder_equiv] ] ] ].
+  - destruct benv'.
+    eapply encoder_OK; eauto.
+  - simpl in *.
+    eapply encoder_OK; eauto.
+Defined.
+
+(* Here are the expected correctness lemmas for synthesized functions. *)
+Lemma CorrectDecodeEncode'
+      {S T} {cache : Cache.Cache}
+      {monoid : Monoid T}
+  : forall Invariant
+           (FormatSpec : Specs.FormatM S T)
+           (encoder : Specs.CorrectEncoderFor FormatSpec)
+           (decoder : Specs.CorrectDecoderFor Invariant FormatSpec),
+    forall a envE envD b envE',
+      Cache.Equiv envE envD
+      -> Invariant a
+      -> snd (proj1_sig decoder) envD
+      -> projT1 encoder a envE = Some (b, envE')
+      -> forall ext, exists envD',
+          fst (proj1_sig decoder) (mappend b ext) envD = Some (a, ext, envD').
+Proof.
+  intros.
+  destruct encoder as [encoder encoder_OK].
+  destruct decoder as [decoder [Inv [decoder_OK Inv_cd] ] ]; simpl in *.
+  specialize (proj1 (encoder_OK a envE) _ H2); intro.
+  specialize (decoder_OK Inv_cd).
+  destruct decoder_OK as [decoder_OK _].
+  unfold Specs.cache_inv_Property in Inv_cd.
+  eapply decoder_OK  with (ext := ext) in H3; eauto.
+  destruct H3 as [? [? ?] ]; intuition.
+  subst; eauto.
+Qed.
+
 (* Here are the expected correctness lemmas for optimized versions of the synthesized functions. *)
 Lemma CorrectDecodeEncode
       {A} {cache : Cache.Cache}
@@ -26,30 +80,163 @@ Lemma CorrectDecodeEncode
       Cache.Equiv ce cd
       -> Invariant a
       -> snd (projT1 (projT2 decoder)) cd
-      -> forall cd' idx ce' v',
+      -> forall idx ce' v',
           projT1 encoder sz v 0 a ce = Some (v', idx, ce')
-          -> (projT1 decoder sz) v' 0 cd = Some (a, idx, cd').
+          -> exists cd' idx',
+            (projT1 decoder sz) v' 0 cd = Some (a, idx', cd').
 Proof.
   intros.
-  destruct encoder as [aligned_encoder aligned_encoder_OK].
-  destruct aligned_encoder_OK as [encoder [encoder_OK [padding_OK encoder_equiv] ] ].
-  destruct decoder as [aligned_decoder [ [decoder Inv] [ [Inv' [decoder_OK Inv_cd] ] decoder_equiv ] ] ]; simpl in *.
-  specialize (decoder_OK Inv_cd).
-Abort.
-(* specialize (encoder_OK ce _ (Core.ReturnComputes _)) .
-  destruct (encoder_equiv ce 0) as [? [? ?] ].
-  specialize (H3 (padding_OK _)).
+  destruct (projT1 (projT2 encoder) a ce) as [ [? ?] | ] eqn: ?.
+  - generalize Heqo; intro.
+    eapply (@CorrectDecodeEncode' _ _ _ _ _ _
+                                  (CorrectAlignedEncoder2CorrectEncoder _ encoder)
+                                  (CorrectAlignedDecoder2CorrectDecoder _ _ decoder))
+      in Heqo; eauto.
+    destruct Heqo.
+    simpl in H3.
+    pose proof (projT2 (projT2 encoder)); simpl in *.
+    destruct H4.
+    pose proof (proj1 H5 _ _ _ _ Heqo0).
+    assert (numBytes b <= sz)%nat.
+    { destruct (Compare_dec.le_gt_dec (8 + 8 * sz) (length_ByteString b + 8 * 0)); eauto.
+      apply @proj2 in H5.
+      eapply proj2 in H5.
+      eapply proj1 in H5.
+      specialize (H5 _ _ _ v Heqo0 l).
+      congruence.
+      unfold length_ByteString in g.
+      rewrite H6 in g.
+      unfold gt in g.
+      Omega.omega.
+    }
+    apply @proj2 in H5.
+    eapply proj1 in H5.
+    generalize H7; intros H7'.
+    assert (numBytes b + (sz - numBytes b) = sz) as sz_eq by Omega.omega.
+    eapply (build_aligned_ByteString_eq_split _ _ v) in H7.
+    instantiate (1 := sz_eq) in H7.
+    eapply (build_aligned_ByteString_eq_split _ _ v') in H7'.
+    instantiate (1 := sz_eq) in H7'.
+    specialize (H5 _ _ Heqo0 H6 (Vector.nil _) (fst (Vector_split _ _ (Guarded_Vector_split (numBytes b) sz v))) _
+                   (snd (Vector_split _ _ (Guarded_Vector_split (numBytes b) sz v)))).
+    destruct H5 as [? [? ?] ].
+    simpl in *.
+    rewrite <- Vector_split_append in H5.
+    pose proof mempty_left; simpl in H9.
+    rewrite IPChecksum.build_aligned_ByteString_nil, H9 in H8.
+    symmetry in H8.
+    destruct (build_aligned_ByteString_split _ _ _ H8).
+    symmetry in H8.
+    rewrite H10 in H8 at 1.
+    rewrite <- build_aligned_ByteString_append in H8.
+    subst.
+    assert (numBytes b + (sz - numBytes b) - (sz - numBytes b) = numBytes b) by Omega.omega.
+    revert x1 H8 H10.
+    rewrite H11; intros.
+    assert (Some ((Guarded_Vector_split (numBytes b) sz v'), idx, ce') = Some
+                                                                           (Vector.append x1
+                                                                                          (snd (Vector_split (numBytes b) (sz - numBytes b) (Guarded_Vector_split (numBytes b) sz v))),
+                                                                            numBytes b, c)).
+    apply build_aligned_ByteString_inj in H8; subst.
+    apply build_aligned_ByteString_inj in H7; subst.
+    apply build_aligned_ByteString_inj in H7'; subst.
+    revert H2.
+    rewrite H7 at 1.
+    rewrite H7' at 1.
+    simpl.
+    simpl in *; unfold ByteBuffer.t in H5.
+    rewrite <- H5.
+    rewrite <- sz_eq.
+    simpl; unfold ByteBuffer.t, Core.char; intros.
+    rewrite <- H2.
+    reflexivity.
+    injection H12; intros; subst; clear H12.
+    instantiate (1 := build_aligned_ByteString (snd (Vector_split (numBytes b) (sz - numBytes b) (Guarded_Vector_split (numBytes b) sz v)))) in H3.
+    apply build_aligned_ByteString_inj in H7'; subst.
+    rewrite H10 in H3 at 1.
+    rewrite <- build_aligned_ByteString_append in H3.
+    rewrite <- H15 in H3.
+    pose proof (proj2 (projT2 (projT2 decoder))).
+    eapply H12 in H3.
+    simpl in H3; destruct H3.
+    eexists _, _.
+    rewrite <- H3.
+    rewrite H7' at 1.
+    generalize sz_eq v'; clear; intros.
+    rewrite <- sz_eq; simpl; reflexivity.
+  - pose proof (projT2 (projT2 encoder)); simpl in *.
+    destruct H3 as [? [? ?] ].
+    specialize (H5 ce a 0); intuition.
+    eapply H9 in Heqo.
+    rewrite Heqo in H2; discriminate.
+Qed.
 
-  destruct decoder_equiv.
-
-  specialize (encoder_OK a ce _ (ReturnComputes _)) .
-  destruct decoder_OK as [decoder_OK _].
-  destruct (encoder a ce) as [bin ce'].
-  unfold cache_inv_Property in Inv_cd.
-  eapply decoder_OK  with (ext := mempty) in encoder_OK; eauto.
-  destruct_ex; intuition.
-  rewrite mempty_right in H3; eauto.
-Qed. *)
+Lemma CorrectEncodeDecode
+      {S}
+      {cache : Cache.Cache}
+  : forall Invariant
+           (FormatSpec : Specs.FormatM S ByteString)
+           (decoder : CorrectAlignedDecoderFor Invariant FormatSpec),
+    forall sz v' ce cd cd' s idx',
+      Cache.Equiv ce cd
+      -> snd (projT1 (projT2 decoder)) cd
+      -> (projT1 decoder sz) v' 0 cd = Some (s, idx', cd')
+      -> Invariant s /\
+         exists ce' (v1 : Vector.t (word 8) idx') (v2 : Vector.t (word 8) (sz - idx')) H,
+           Guarded_Vector_split idx' sz v' = eq_rect _ _ (Vector.append v1 v2) _ H
+           /\ Cache.Equiv ce' cd' /\ FormatSpec s ce (build_aligned_ByteString v1, ce').
+Proof.
+  intros.
+  pose proof (Specs.CorrectEncodeDecode _ _ (CorrectAlignedDecoder2CorrectDecoder _ _ decoder)).
+  simpl in *.
+  destruct (fst (projT1 (projT2 decoder)) (build_aligned_ByteString v') cd)
+    as [ [ [? ?] ?] | ] eqn: ?.
+  - specialize (H2 _ _ _ _ _ _ H H0 Heqo);
+      destruct H2 as [? [? [? [? [? ?] ] ] ] ].
+    pose proof (proj2 (projT2 (projT2 decoder))).
+    destruct H6 as [_ [? [? ?] ] ].
+    specialize (H8 _ _ _ Heqo).
+    specialize (H6 _ _ _ _ _ Heqo).
+    destruct H8 as [? [? ?] ].
+    rewrite H8 in H1; injection H1; intros; subst.
+    intuition.
+    assert (sz >= numBytes b)%nat.
+    { revert H6; unfold length_ByteString; simpl.
+      generalize (paddingOK b); clear; intros; Omega.omega. }
+    assert (sz - numBytes b + (sz - (sz - numBytes b)) = sz - numBytes b + (sz - (sz - numBytes b))).
+    Omega.omega.
+    assert ((sz - (sz - numBytes b)) = numBytes b) by Omega.omega.
+    eexists _, (fst (Vector_split _ _ (Guarded_Vector_split (sz - numBytes b) sz v'))),
+    (snd (Vector_split _ _ (Guarded_Vector_split (sz - numBytes b) sz v'))), H12;
+      intuition eauto.
+    rewrite <- Vector_split_append.
+    revert H12.
+    destruct H13; intros.
+    clear.
+    intros; rewrite <- Eqdep_dec.eq_rect_eq_dec; eauto.
+    decide equality.
+    destruct (build_aligned_ByteString_split' _ _ _ H9).
+    rewrite H14 in H3.
+    destruct (build_aligned_ByteString_split _ _ _ H3).
+    subst.
+    rewrite <- build_aligned_ByteString_append in H3.
+    rewrite build_aligned_ByteString_eq_split' with (n := sz - numBytes b) in H3; eauto.
+    replace (build_aligned_ByteString
+       (fst
+          (Vector_split (sz - numBytes b) (sz - (sz - numBytes b)) (Guarded_Vector_split (sz - numBytes b) sz v'))))
+               with (build_aligned_ByteString x3); eauto.
+    revert x2 x3 H3 H5 H14.
+    generalize (Guarded_Vector_split (sz - numBytes b) sz v').
+    rewrite H13.
+    intros.
+    apply build_aligned_ByteString_inj in H3; subst.
+    rewrite <- Vector_append_split_fst; eauto.
+    clear; Omega.omega.
+  - pose proof (proj2 (projT2 (projT2 decoder))).
+    destruct H3 as [_ [? [? ?] ] ].
+    apply H4 in Heqo.
+    congruence.
+Qed.
 
 (* Various Constants that clients should never simplify. *)
 Global Arguments split1 : simpl never.
