src/Narcissus/Examples/NetworkStack/TCP_Packet.v
@@ -103,6 +103,9 @@ Section TCPPacketDecoder.
     CorrectAlignedEncoderFor TCP_Packet_Format.
   Proof.
     synthesize_aligned_encoder.
+    Grab Existential Variables.
+    eauto.
+    eauto.
   Defined.
 
   (* Step Two: Extract the encoder function, and have it start encoding
